`SimpleIter` example ITree proof and reorganize files

LeanBoogie/Boog.lean
@@ -1,5 +1,8 @@
 import Std
 import Aesop
+import LeanBoogie.ITree
+import LeanBoogie.Notation
+import LeanBoogie.Iter
 
 namespace Boogie
 
@@ -10,84 +13,73 @@ open Std (HashSet HashMap)
   Tracks values of boogie variables during execution.
 -/
 
+
 /-- Assigns values to every variable. Ideally you'd want `(v : String) -> v ∈ ValidVars -> Int`. -/
 abbrev BoogieState := String -> Int
+
+def BoogieState.update (v : String) (val : Int) : BoogieState -> BoogieState :=
+  fun σ v' => if _h : v' = v then val else σ v'
 instance : EmptyCollection BoogieState := ⟨fun _ => 0⟩
 
+
 /-- State monad during execution of boogie programs. Assigns values to every variable. -/
-abbrev Boog : Type -> Type := StateM BoogieState
+abbrev Boog (E : Type) : Type -> Type := StateT BoogieState (ITree E)
 
-def Boog.skip : Boog Unit := pure ()
-def Boog.seq (a b : Boog Unit) : Boog Unit := a >>= (fun _ => b)
+def Boog.read (v : String) : Boog E Int := fun σ => pure (σ v, σ)
+def Boog.write (v : String) (val : Int) : Boog E Unit := fun σ => pure ((), BoogieState.update v val σ)
+/-- Apply a pure function to a variable. Useful for simple operations such as increments, setting to zero, etc. -/
+def Boog.update (v : String) (f : Int -> Int) : Boog E Unit
+  := Boog.read v >>= fun x => Boog.write v (f x)
 
-def Boog.get (v : String) : Boog Int := do return (<- getThe BoogieState) v
-def Boog.set (v : String) (e : Boog Int) : Boog Unit := do
-  let val <- e
-  modifyThe BoogieState
-      (fun f x => if x = v then val else f x)
 
-/-- This is a little ugly, because lean `if` actually takes a (decidable) `Prop`, not a `Bool` -/
-def Boog.ifthenelse (c : Boog Bool) (t e : Boog Unit) : Boog Unit := do
-  if <- c then t else e
+/- ## Helpers for writing imperative programs.  -/
 
-def Boog.ifthen (c : Boog Bool) (t : Boog Unit) : Boog Unit := do
-  if <- c then t
+def Boog.iter (f : A -> Boog E (A ⊕ B)) : A -> Boog E B := sorry
+instance : Iter (Boog E) := ⟨Boog.iter⟩
+
+def Boog.skip : Boog E Unit := pure ()
+def Boog.seq (a b : Boog E Unit) : Boog E Unit := a >>= (fun () => b)
+instance : Seqi (Boog E Unit) := ⟨Boog.seq⟩
+
+def Boog.case (t e : Boog E A) : Bool -> Boog E A
+| true => t
+| false => e
+
+def Boog.ite (c : Boog E Bool) (t e : Boog E A) : Boog E A :=
+  c >>= Boog.case t e
+
+abbrev Boog.pure : A -> Boog E A := Pure.pure
+abbrev Boog.bind : (Boog E A) -> (A -> Boog E B) -> Boog E B := Bind.bind
 
 /-- Actually execute a boogie program, starting with every variable being 0-initialized. -/
-def runBoogie (m : Boog Unit) : BoogieState :=
+def Boog.run (m : Boog Empty Unit) (fuel : Nat) : Option BoogieState :=
   let s₀ : BoogieState := (fun _ => 0)
-  let ((), s') := StateT.run m s₀
-  s'
+  let stuff := StateT.run m s₀
+  let ⟨_, ret⟩ := ITree.run stuff Empty.elim fuel
+  ret.map Prod.snd
 
-/-
-  ## Helper lemmas
-  Elaborated Boogie programs are quite noisy, and not structured in a way that Lean-Auto can deal
-  with very well. So here we define a bunch of lemmas which (hopefully) bring elaborated Boogie
-  programs into a shape that SMT solvers can deal with.
--/
+/-- Equivalence up-to-tau, but adapted for the `Boog` monad. -/
+def EuttB (b1 : Boog E A) (b2 : Boog E A) : Prop := ∀σ : BoogieState, Eutt (b1 σ) (b2 σ)
+infixr:20 " ~=~ " => EuttB
 
-theorem bind_eq2 (a: Boog A) (b: A -> Boog B) : (a >>= b : Boog B) = fun s => let x := a s ; b x.fst x.snd
-:= by
-  unfold bind Monad.toBind StateT.instMonad StateT.bind
-  simp
+axiom EuttB.eq {E A : Type} {x y : Boog E A} : EuttB x y -> x = y
 
-@[aesop unsafe] theorem one_var {t1 t2 : String -> Int} (x : String)
-  (h_x     : t1 x = t2 x)
-  (h_other : (∀v, ¬ v = x -> t1 v = t2 v))
-  : ∀v, t1 v = t2 v
-  := by intro v; if h : x = v then exact h ▸ h_x else aesop
+theorem Boog.ite_push_state [Decidable c] {t e : Boog E A}
+  : (if c then t else e) σ ~~ (if c then t σ else e σ)
+  := by split; repeat exact Eutt.refl _
 
-@[simp]
-theorem ite_bind:
-  ∀ [Monad m]
-    {c : Bool}
-    {m1 m2 : m a}
-    {k : a -> m b},
-   (if c then m1       else m2      ) >>= k
-  = if c then m1 >>= k else m2 >>= k
-  := by aesop
+theorem Boog.bind_push_state {a : Boog E A} {b : A -> Boog E B}
+  : (a >>= b) σ ~~ (a σ >>= fun res => b res.fst res.snd)
+  := sorry
 
-@[simp]
-theorem var_congr_ite
-  [Decidable c]
-  (x : String)
-  {t e t' e' : Boog A}
-  (h_t :   c -> (t st).2 x = (t' st).2 x)
-  (h_e : ¬ c -> (e st).2 x = (e' st).2 x)
-  : ((if c then t else e) st).2 x = ((if c then t' else e') st).2 x
-  := by aesop
+def Boog.while_ (c : Boog E Bool) (body : Boog E Unit) : Boog E Unit :=
+  Boog.iter
+    (fun () => Boog.ite c
+      (do body; return .inl ())
+      (return .inr ()))
+    ()
 
-@[simp]
-theorem state_congr_ite [Decidable c] {t e : Boog A}
-  : (if c then t else e) st = (if c then t st else e st)
-  := by aesop
-
-@[simp]
-theorem state_proj_congr_ite [Decidable c] {tst est :(A × S)}
-  : (if c then tst else est).2 = (if c then (tst).2 else (est).2)
-  := by aesop
-
-@[simp]
-theorem state_var_ite_congr [Decidable c] {t e : String -> Int}
-  : (if c then t else e) v = (if c then t v else e v)
+@[simp] theorem ite_bind [Monad m] [Decidable c] {m1 m2 : m a} {k : a -> m b}
+  : (if c then m1       else m2      ) >>= k
+  =  if c then m1 >>= k else m2 >>= k
   := by aesop
