LeanBoogie/ITree/ITree.lean
@@ -119,7 +119,95 @@ def run (t : ITree E A) (f : E -> Ans) : Nat -> (List E) × Option A
     let (evs, ret) := run t f n
     exact (e :: evs, ret)
 
-abbrev KTree (E A B : Type) : Type := A -> ITree E B
+/-- We use theorems from the ITree paper without proof, for now. Give a justification or source in `ref`. -/
+axiom trustITree {P : Prop} (ref : String) : P
+
+/-
+  ## `ITree` forms a monad
+-/
+
+def pure (a : A) : ITree E A := .ret a
+
+def bind (ta : ITree E A) (tb : A -> ITree E B) : ITree E B :=
+  ITree.corec (β := Sum (ITree E A) (ITree E B)) (fun x =>
+    match x with
+    | .inl ta =>
+      match ta.dest with
+      | .ret (a : A) =>
+        let tb : ITree E B := tb a
+        let ret : ITree.Base E B (ITree E B) := tb.dest
+        let ret : ITree.Base E B (ITree E A ⊕ ITree E B) := MvFunctor.map (F := TypeFun.ofCurried (n := 3) ITree.Base) Base.Inr ret
+        ret
+      | .tau t => .tau (.inl t)
+      | .vis e k => .vis e (fun x => .inl (k x))
+    | .inr b => Base.replay b Sum.inr
+  ) (Sum.inl ta)
+
+instance : Monad (ITree E) where
+  pure := pure
+  bind := bind
+
+instance : LawfulFunctor (ITree E) where
+  map_const := sorry
+  id_map := sorry
+  comp_map := sorry
+
+instance : LawfulMonad (ITree E) where
+  seqLeft_eq := sorry
+  seqRight_eq := sorry
+  pure_seq := sorry
+  bind_pure_comp := sorry
+  bind_map := sorry
+  pure_bind := sorry
+  bind_assoc := sorry
+
+
+/-
+  ## Iter
+-/
+
+/-- Repeat a computation until it returns `B`.
+
+  From the ITrees paper, page 12:
+  ```
+  CoFixpoint iter (body : A → itree E (A + B)) : A → itree E B :=
+    fun a ⇒ ab <- body a ;;
+      match ab with
+      | inl a ⇒ Tau (iter body a)
+      | inr b ⇒ Ret b
+      end.
+  ``` -/
+def iter (body : A -> ITree E (A ⊕ B)) (a₀ : A) : ITree E B := sorry
+  -- ITree.corec (fun (x : A ⊕ ITree E (B)) =>
+  --   match x with
+  --   | .inl a =>
+  --     -- Run the body, if it returned `a` we iter again, if it returned `b` we are done.
+  --     let res : ITree E (A ⊕ B) := bind (body a) (fun ab =>
+  --       match ab with
+  --       | .inl a => .ret (.inl a)
+  --       | .inr b => .ret (.inr b)
+  --     )
+  --     match res.dest with
+  --     -- | .ret (a : A ⊕ B) => .ret sorry
+  --     | .ret (.inl a) => .tau (.inl a) -- call `iter body a`
+  --     | .ret (.inr b) => .ret b -- we are done
+  --     | .tau (t : ITree E _) => .tau (.inr t)
+  --     | .vis e k => sorry
+  --   | .inr b => Base.replay b .inr
+  -- ) (Sum.inl a₀)
+
+
+/--
+  Definition loop (body : C + A → itree E (C + B)) : A → itree E B :=
+    fun a ⇒ iter (fun ca ⇒
+      cb <- body ca ;;
+      match cb with
+      | inl c ⇒ Ret (inl (inl c))
+      | inr b ⇒ Ret (inr b)
+      end) (inr a).
+-/
+def loop (body : Sum C A -> ITree E (Sum C B)) (a : A) : ITree E B := sorry
+
 
 -- # Experimentation:
 
