Examples/SimpleIter.lean
@@ -1,0 +1,64 @@
+-- import LeanBoogie.BoogieDsl
+import LeanBoogie.ITree
+import LeanBoogie.Boog
+import LeanBoogie.Mem
+import Auto
+import Aesop
+
+open Boogie ITree
+
+set_option auto.smt true
+set_option trace.auto.smt.printCommands true
+set_option trace.auto.smt.result true
+set_option trace.auto.printLemmas true
+set_option auto.smt.trust true
+set_option auto.smt.solver.name "z3"
+set_option pp.fieldNotation.generalized false
+
+-- Very simple example which can be proven using unrolling or a congruence on the while loop
+
+def p1 : ITree MemEv Unit := do
+  Mem.write "i" 0
+  while_ (return (<- Mem.read "i") < 3) do
+    Mem.update "i" (. + 1)
+    Mem.update "x" (. + 2)
+  Mem.write "i" 0 -- need to set `i` to 0 afterwards, otherwise the programs compute the same `x` but not `i`.
+
+def p2 : ITree MemEv Unit := do
+  Mem.write "i" 0
+  while_ (return (<- Mem.read "i") < 6) do
+    Mem.update "x" (. + 1)
+    Mem.update "i" (. + 1)
+  Mem.write "i" 0
+
+example : EuttB (interp p1) (interp p2) := by
+  rw [p1, p2]
+  -- 1. unroll loops
+  conv => lhs; rw [Eutt.eq while_unroll1, Eutt.eq while_unroll1, Eutt.eq while_unroll1, Eutt.eq while_unroll1, Eutt.eq while_unroll1]
+  conv => rhs; rw [Eutt.eq while_unroll1, Eutt.eq while_unroll1, Eutt.eq while_unroll1, Eutt.eq while_unroll1, Eutt.eq while_unroll1, Eutt.eq while_unroll1, Eutt.eq while_unroll1, Eutt.eq while_unroll1]
+
+  -- 2. Push `interp` inwards as far as possible,
+  -- this will change `ITree.{pure, bind, iter, ite, read, write}`
+  -- into `Boog.{pure, bind, iter, ite, read, write}`
+  simp [EuttB.eq interp_bind, EuttB.eq interp_write, EuttB.eq interp_ite, EuttB.eq interp_pure,
+    Mem.update, EuttB.eq interp_write, EuttB.eq interp_read, skip]
+  -- Our goal is now of form `b1 b2 : (S -> ITree ∅ (A × S)) ⊢ ∀σ:S, Eutt (b1 σ) (b2 σ)`, with the predominant `bind` being `Boog.bind`.
+
+  -- 3. Push state `σ` inwards as far as possible. This allows us to apply `pure_bind` and obtain
+  -- a pure state transition function, because we no longer have any relevant coinduction.
+  -- Nonetheless, this causes the predominant `bind` to become `ITree.bind` yet again (`Boog.read v : Boog ..`, but `Boog.read v σ : ITree ..`).
+  -- However, we know that `ITree.bind (Boog.read v σ) k` is actually `ITree.bind (ITree.pure (σ v, σ)) k`, which simplifies to `k (σ v) σ` via `pure_bind`. Similar for `.write`.
+  intro σ
+  simp only [Eutt.eq Boog.bind_push_state, Eutt.eq Boog.ite_push_state]
+  simp only [Boog.read, Boog.write, BoogieState.update.eq_unfold]
+  simp only [pure_bind, Nat.ofNat_pos, dite_eq_ite, ↓reduceDIte, ↓reduceIte, String.reduceEq, zero_add, Nat.one_lt_ofNat, Int.reduceAdd, Int.reduceLT, lt_self_iff_false]
+  simp_all only [↓reduceIte]
+
+  dsimp [Pure.pure, ITree.pure]
+  -- Our goal is now of form `σ : S ⊢ .ret (a, f σ) = .ret (b, g σ)`
+  apply Eutt.ret_congr
+  congr 1
+  unfold BoogieState at σ
+  unfold BoogieState
+  -- 4. Solve by auto :)
+  auto
