LeanBoogie/ITree/Imp.lean
@@ -1,0 +1,30 @@
+import LeanBoogie.ITree.ITree
+import LeanBoogie.ITree.Eutt
+import LeanBoogie.Notation
+import LeanBoogie.Iter
+
+namespace ITree
+
+/- # Convenience functions for writing imperative programs -/
+
+def skip : ITree E Unit := Pure.pure ()
+def spin : ITree E A := corec (fun n => .tau n) 0
+def seq (a b : ITree E Unit) : ITree E Unit := bind a (fun () => b)
+instance : Seqi (ITree E Unit) := ⟨ITree.seq⟩
+def trigger (e : E) : ITree E Int := .vis e .ret
+def ite (c : ITree E Bool) (t e : ITree E A) : ITree E A := bind c (fun c => if c then t else e)
+abbrev ifthen (c : ITree E Bool) (t : ITree E Unit) : ITree E Unit := ite c t skip
+
+def while_ (c : ITree E Bool) (body : ITree E Unit) : ITree E Unit :=
+  ITree.iter
+    (fun () => ITree.ite c
+      (do body; return .inl ())
+      (return .inr ()))
+    ()
+
+theorem while_unroll1 : while_ c f ~~ ITree.ite c (do f; while_ c f) skip := by sorry
+
+/-- Decide the proposition, spin forever if false. -/
+def assume (φ : Prop) [Decidable φ] : ITree E Unit := if φ then skip else spin
+
+end ITree
