LeanBoogie/Mem.lean
@@ -1,0 +1,73 @@
+import LeanBoogie.ITree
+import LeanBoogie.Boog
+import LeanBoogie.Notation
+
+namespace Boogie
+
+/-
+  # Memory effect
+-/
+
+example : Ans = Int := rfl -- currently our ITrees have the answer type hardcoded as Int.
+
+/-- Memory events: Reading or writing of a variable. -/
+inductive MemEv
+| read  : String        -> MemEv
+| write : String -> Int -> MemEv
+deriving Repr
+
+-- abbrev Mem : Type -> Type := ITree MemEv
+
+def Mem.read (v : String)            : ITree MemEv Int  := .vis (.read v) (fun ans => .ret ans)
+def Mem.write (a : String) (b : Int) : ITree MemEv Unit := .vis (.write a b) (fun _unit => .ret ())
+/-- Apply a pure function to a variable. Useful for simple operations such as increments, setting to zero, etc. -/
+def Mem.update (v : String) (f : Int -> Int) : ITree MemEv Unit
+  := Mem.read v >>= fun x => Mem.write v (f x)
+
+/-
+  # Interpreting memory
+-/
+
+/-- Transforms memory events into state monad actions. -/
+def interp (tm : ITree MemEv A) : Boog Empty A := fun s₀ =>
+  ITree.corec (fun ⟨tm, s⟩ =>
+    match tm.dest with
+    | .ret a => .ret (a, s)
+    | .tau t => .tau (t, s)
+    | .vis (.read v) k => .tau ⟨k (s v), s⟩
+    | .vis (.write v val) k => .tau ⟨k default, s.update v val⟩ -- TODO: Instead of `default : Int`, this should be `() : Unit` once the QPF ITree limitation is gone.
+  ) (tm, s₀)
+
+-- def interpk (k : KTree MemEv A B) : Book Empty A B := fun a => interp (k a)
+
+theorem interp_pure : interp (pure x) ~=~ pure x := sorry
+
+theorem interp_bind {ta : ITree MemEv A} {tb : A -> ITree MemEv B}
+  : interp (bind ta tb) ~=~ bind (interp ta) (fun a => interp (tb a))
+  := sorry
+
+
+/-- Convenience mix of `interp_bind` and `bind_state_pull`. -/
+theorem interp_bind_pull {ta : ITree MemEv A} {tb : A -> ITree MemEv B}
+  : interp (ITree.bind ta tb) s ~~ ITree.bind (interp ta s) (fun x => interp (tb x.1) x.2)
+  := sorry
+
+
+theorem interp_iter {body : A -> ITree MemEv (A ⊕ B)} {a₀ : A}
+  : interp (ITree.iter body a₀) ~=~ Boog.iter (fun (a : A) => interp (body a)) a₀
+  := sorry
+
+-- theorem interpk_iter {body : A -> ITree MemEv (A ⊕ B)} {a₀ : A}
+--   -- : ∀a, ∀s, interpk (ITree.iter body) a s ~~ Boog.iter (interpk body) a s
+--   : interpk (ITree.iter body) ~~=~~ Boog.iter (interpk body)
+--   := by sorry
+
+theorem interp_read : interp (Mem.read x) ~=~ Boog.read x := sorry
+theorem interp_write : interp (Mem.write x val) ~=~ (Boog.write x val) := sorry
+
+theorem interp_ite : interp (ITree.ite c t e) ~=~ (do let c <- interp c; if c then interp t else interp e :) := sorry
+
+-- theorem interp_cat {f : KTree MemEv A B} {g : KTree MemEv B C}
+--   : interp (f a >>> g) ~~ (interp f >>> interpK g) a := sorry
+-- theorem interpK_cat {f : KTree MemEv A B} {g : KTree MemEv B C}
+--   : interpK (f >>> g) a ~~~ (interpK f >>> interpK g) a := sorry
