LeanBoogie/Notation.lean
@@ -1,0 +1,10 @@
+
+/-- Two imperative programs executed after one another. Provides the `;; ` notation. -/
+class Seqi (A : Type) where
+  seqi : A -> A -> A
+infixl:20 ";; " => Seqi.seqi
+
+/-- Concatenation of continuations. Provides the `>>>` notation. -/
+class Cat (K : Type -> Type -> Type) where
+  cat : K A B -> K B C -> K A C
+infixl:75 " >>> " => Cat.cat
